src/coq/Theory/InterpreterMCFG.v
@@ -57,21 +57,20 @@ Module Type MCFGTheory (IS : InterpreterStack) (TOP : LLVMTopLevel IS).
 
     Ltac go_in H :=
       repeat match goal with
-             | |- context [interp_intrinsics (ITree.bind _ _)] => rewrite interp_intrinsics_bind in H
-             | |- context [interp_global (ITree.bind _ _)] => rewrite interp_global_bind in H
-             | |- context [interp_local_stack (ITree.bind _ _)] => rewrite interp_local_stack_bind in H
-             | |- context [interp_memory (ITree.bind _ _)] => rewrite interp_memory_bind in H
-             | |- context [interp_intrinsics (trigger _)] => rewrite interp_intrinsics_trigger in H; cbn in H; rewrite ?subevent_subevent in H
-             | |- context [interp_global (trigger _)] => rewrite interp_global_trigger in H; cbn in H; rewrite ?subevent_subevent in H
-             | |- context [interp_local_stack (trigger _)] => rewrite interp_local_stack_trigger in H; cbn in H; rewrite ?subevent_subevent in H
-             | |- context [ITree.bind (ITree.bind _ _) _] => rewrite bind_bind in H
-             | |- context [interp_intrinsics (Ret _)] => rewrite interp_intrinsics_ret in H
-             | |- context [interp_global (Ret _)] => rewrite interp_global_ret in H
-             | |- context [interp_local_stack (Ret _)] => rewrite interp_local_stack_ret in H
-             | |- context [interp_memory (Ret _)] => rewrite interp_memory_ret in H
-             | |- context [ITree.bind (Ret _) _] => rewrite bind_ret_l in H
+             | H: context [interp_intrinsics (ITree.bind _ _)] |- _ => rewrite interp_intrinsics_bind in H
+             | H: context [interp_global (ITree.bind _ _)] |- _ => rewrite interp_global_bind in H
+             | H: context [interp_local_stack (ITree.bind _ _)] |- _ => rewrite interp_local_stack_bind in H
+             | H: context [interp_memory (ITree.bind _ _)] |- _ => rewrite interp_memory_bind in H
+             | H: context [interp_intrinsics (trigger _)] |- _ => rewrite interp_intrinsics_trigger in H; cbn in H; rewrite ?subevent_subevent in H
+             | H: context [interp_global (trigger _)] |- _ => rewrite interp_global_trigger in H; cbn in H; rewrite ?subevent_subevent in H
+             | H: context [interp_local_stack (trigger _)] |- _ => rewrite interp_local_stack_trigger in H; cbn in H; rewrite ?subevent_subevent in H
+             | H: context [ITree.bind (ITree.bind _ _) _] |- _ => rewrite bind_bind in H
+             | H: context [interp_intrinsics (Ret _)] |- _ => rewrite interp_intrinsics_ret in H
+             | H: context [interp_global (Ret _)] |- _ => rewrite interp_global_ret in H
+             | H: context [interp_local_stack (Ret _)] |- _ => rewrite interp_local_stack_ret in H
+             | H: context [interp_memory (Ret _)] |- _ => rewrite interp_memory_ret in H
+             | H: context [ITree.bind (Ret _) _] |- _ => rewrite bind_ret_l in H
              end.
-
 
   End MCFGTactics.
 
